backends/lean/Aeneas/Std/Scalar/WrappingOps/Add.lean
@@ -9,74 +9,48 @@ open Result Error ScalarElab
 # Wrapping Add
 -/
 
-def UScalar.wrapping_add {ty} (x y : UScalar ty) : UScalar ty := ⟨ x.toBitVec + y.toBitVec ⟩
-
-def IScalar.wrapping_add {ty} (x y : IScalar ty) : IScalar ty := ⟨ x.toBitVec + y.toBitVec ⟩
-
-uscalar @[step_pure_def]
-def «%S».wrapping_add (x y : «%S») : «%S» := @UScalar.wrapping_add UScalarTy.«%S» x y
-
-iscalar @[step_pure_def]
-def «%S».wrapping_add (x y : «%S») : «%S» := @IScalar.wrapping_add IScalarTy.«%S» x y
+scalar @[step_pure_def]
+def «%S».wrapping_add (x y : «%S») : «%S» := ⟨ x.toBitVec + y.toBitVec ⟩
 
 /- [core::num::{_}::wrapping_add] -/
-uscalar @[step_pure_def]
-def core.num.«%S».wrapping_add : «%S» → «%S» → «%S» := @UScalar.wrapping_add UScalarTy.«%S»
+scalar @[step_pure_def]
+def core.num.«%S».wrapping_add : «%S» → «%S» → «%S» := _root_.Aeneas.Std.«%S».wrapping_add
 
-/- [core::num::{_}::wrapping_add] -/
-iscalar @[step_pure_def]
-def core.num.«%S».wrapping_add : «%S» → «%S» → «%S»  := @IScalar.wrapping_add IScalarTy.«%S»
-
-@[simp, bvify] theorem UScalar.wrapping_add_toBitVec_eq {ty} (x y : UScalar ty) :
-  (wrapping_add x y).toBitVec = x.toBitVec + y.toBitVec := by
-  simp only [wrapping_add]
-
-uscalar @[simp, bvify, grind =, agrind =] theorem «%S».wrapping_add_bv_eq (x y : «%S») :
+uscalar @[simp, bvify, grind =, agrind =] theorem «%S».wrapping_add_toBitVec_eq (x y : «%S») :
   («%S».wrapping_add x y).toBitVec = x.toBitVec + y.toBitVec := by
   simp [«%S».wrapping_add]
 
-uscalar @[simp, bvify, grind =, agrind =] theorem core.num.«%S».wrapping_add_bv_eq (x y : «%S») :
+uscalar @[simp, bvify, grind =, agrind =] theorem core.num.«%S».wrapping_add_toBitVec_eq (x y : «%S») :
   (core.num.«%S».wrapping_add x y).toBitVec = x.toBitVec + y.toBitVec := by
   simp [core.num.«%S».wrapping_add]
 
-@[simp, bvify] theorem IScalar.wrapping_add_toBitVec_eq {ty} (x y : IScalar ty) :
-  (wrapping_add x y).toBitVec = x.toBitVec + y.toBitVec := by
-  simp only [wrapping_add]
-
-iscalar @[simp, bvify, grind =, agrind =] theorem «%S».wrapping_add_bv_eq (x y : «%S») :
+iscalar @[simp, bvify, grind =, agrind =] theorem «%S».wrapping_add_toBitVec_eq (x y : «%S») :
   («%S».wrapping_add x y).toBitVec = x.toBitVec + y.toBitVec := by
   simp [«%S».wrapping_add]
 
-iscalar @[simp, bvify, grind =, agrind =] theorem core.num.«%S».wrapping_add_bv_eq (x y : «%S») :
+iscalar @[simp, bvify, grind =, agrind =] theorem core.num.«%S».wrapping_add_toBitVec_eq (x y : «%S») :
   (core.num.«%S».wrapping_add x y).toBitVec = x.toBitVec + y.toBitVec := by
   simp [core.num.«%S».wrapping_add]
 
-@[simp] theorem UScalar.wrapping_add_toNat_eq {ty} (x y : UScalar ty) :
-  (wrapping_add x y).toNat = (x.toNat + y.toNat) % (UScalar.size ty) := by
-  simp only [wrapping_add, toNat, size]
-  have : 0 < 2^ty.numBits := by simp
-  have : 2 ^ ty.numBits - 1 + 1 = 2^ty.numBits := by omega
+uscalar @[simp, grind =, agrind =] theorem «%S».wrapping_add_toNat_eq (x y : «%S») :
+  («%S».wrapping_add x y).toNat = (x.toNat + y.toNat) % UScalar.size .«%S» := by
+  simp only [wrapping_add, UScalar.toNat, UScalar.size]
+  have : 0 < 2^«%S».numBits := by simp
+  have : 2 ^ «%S».numBits - 1 + 1 = 2^«%S».numBits := by omega
   simp only [BitVec.toNat_add, toBitVec_toNat]
 
-uscalar @[simp, grind =, agrind =] theorem «%S».wrapping_add_val_eq (x y : «%S») :
-  («%S».wrapping_add x y).toNat = (x.toNat + y.toNat) % (UScalar.size .«%S») :=
-  UScalar.wrapping_add_toNat_eq x y
+uscalar @[simp, grind =, agrind =] theorem core.num.«%S».wrapping_add_toNat_eq (x y : «%S») :
+  (core.num.«%S».wrapping_add x y).toNat = (x.toNat + y.toNat) % UScalar.size .«%S» :=
+  _root_.Aeneas.Std.«%S».wrapping_add_toNat_eq x y
 
-uscalar @[simp, grind =, agrind =] theorem core.num.«%S».wrapping_add_val_eq (x y : «%S») :
-  (core.num.«%S».wrapping_add x y).toNat = (x.toNat + y.toNat) % (UScalar.size .«%S») :=
-  UScalar.wrapping_add_toNat_eq x y
-
-@[simp] theorem IScalar.wrapping_add_toInt_eq {ty} (x y : IScalar ty) :
-  (wrapping_add x y).toInt = Int.bmod (x.toInt + y.toInt) (2^ty.numBits) := by
-  simp only [wrapping_add, toInt, ]
+iscalar @[simp, grind =, agrind =] theorem «%S».wrapping_add_toInt_eq (x y : «%S») :
+  («%S».wrapping_add x y).toInt = Int.bmod (x.toInt + y.toInt) (2^ %BitWidth) := by
+  simp only [wrapping_add, IScalar.toInt]
   simp only [BitVec.toInt_add, toBitVec_toInt_eq]
+  rfl
 
-iscalar @[simp, grind =, agrind =] theorem «%S».wrapping_add_val_eq (x y : «%S») :
-  («%S».wrapping_add x y).toInt = Int.bmod (x.toInt + y.toInt) (2^ %BitWidth) :=
-  IScalar.wrapping_add_toInt_eq x y
-
-iscalar @[simp, grind =, agrind =] theorem core.num.«%S».wrapping_add_val_eq (x y : «%S») :
+iscalar @[simp, grind =, agrind =] theorem core.num.«%S».wrapping_add_toInt_eq (x y : «%S») :
   (core.num.«%S».wrapping_add x y).toInt = Int.bmod (x.toInt + y.toInt) (2^ %BitWidth) :=
-  IScalar.wrapping_add_toInt_eq x y
+  _root_.Aeneas.Std.«%S».wrapping_add_toInt_eq x y
 
 end Aeneas.Std
